proof/garble/prReal.ec
@@ -7,64 +7,233 @@ require import Int.
 require import Bool.
 require import Array.
 require import Logic.
+require import Real.
+require import Distr.
+require import MyRand.
 
-require import Dkc.
+require import MyDkc.
 require import GarbleTools.
 require import Garble.
-require AdvGarble.
+require import AdvGarbleAda.
 
+(*STRANGE VEHAVIOUR :
+module type Ty = {}.
+
+  module M(A:Ty, B:Ty) = {
+fun f() : unit = {}
+}.
+
+
+  module G(A:Ty, B:Ty) = {
+
+    module C = M(A, B)
+
+fun f() : unit = {C.f();}
+  }.
+
+theory T.
+module X : Ty = {}.
+end T.
+
+equiv test : G(T.X, T.X).f ~ G(T.X, T.X).f : true ==> true.
+fun.
+inline M(T.X,T.X).f.
+inline G(T.X, T.X).C.f.
+*)
+
+module RandGarble2 : Rand_t = {
+  fun gen(f:funct, x:input) : random = {
+    var i : int;
+    var g : int;
+    var a : int;
+    var b : int;
+    var t:bool array;
+    var v : bool;
+    var xx : tokens;
+    var tok : token;
+    var n : int;
+    var m : int;
+    var q : int;
+    var aa : w2g;
+    var bb : w2g;
+    var gg : bool g2v;
+    (n, m, q, aa, bb, gg) = f;
+
+    i = 0;
+    while (i < n+q-m-1) {
+      t.[i] = $Dbool.dbool;
+      i = i + 1;
+    }
+    while (i < (getN f)+(getQ f)-1) {
+      t.[i] = false;
+      i = i + 1;
+    }
+
+    g = n;
+    while (g < n+q-1) {
+      a = aa.[g];
+      b = bb.[g];
+      if (a = 0) {
+        v = ! (eval f x i);
+        
+        tok = $DKC.genRandKeyLast (t.[b]);
+        xx = setTok xx g false tok;
+
+        tok = $DKC.genRandKeyLast (evalGate gg.[g] (v,false));
+        xx = setTok xx g (evalGate gg.[g] (v,false)) tok;
+
+        tok = $DKC.genRandKeyLast (!t.[b]);
+        xx = setTok xx g true tok;
+
+        tok = $DKC.genRandKeyLast (evalGate gg.[g] (v,true));
+        xx = setTok xx g (evalGate gg.[g] (v,true)) tok;
+      }
+      g = g + 1;
+    }
+
+    i = 0;
+    while (i < n+q-1) {
+      if (getTok xx i true = void /\ i <> 0) {
+        tok = $DKC.genRandKeyLast (! t.[i]);
+        xx = setTok xx i true tok;
+      }
+      if (getTok xx i false = void) {
+        tok = $DKC.genRandKeyLast (t.[i]);
+        xx = setTok xx i false tok;
+      }
+      i = i + 1;
+    }
+    return xx;
+  }
+}.
 
 
 lemma realEq :
-  forall (ADV <: Garble.Adv{AdvGarble.Adv}),
+  forall (ADV <: Garble.Adv{AdvAda, DKC.Dkc}),
     equiv [
-      Dkc.Game(Dkc.Dkc, AdvGarble.Adv(ADV)).work ~
-      Garble.Game(Garble.PrvInd(RandGarble), ADV).main
+      GameAda(DKC.Dkc, ADV).work ~
+      Garble.Game(Garble.PrvInd(RandGarble2), ADV).main
       : (glob ADV){1} = (glob ADV){2} /\
-      (Dkc.Dkc.b{1}) /\ (AdvGarble.Adv.l{1}=0) ==> res{1} = res{2}
-    ]
+      (DKC.Dkc.b{1}) /\ (AdvAda.l{1}=0) ==> res{1} = res{2}
+    ].
 proof.
 
   intros ADV.
   fun.
-  inline {1} AdvGarble.Adv(ADV).gen_queries.
-  inline {1} AdvGarble.Adv(ADV).get_challenge.
-  inline {1} Dkc.Dkc.preInit.
-  inline {1} Dkc.Dkc.get_challenge.
-  inline {1} Dkc.Dkc.initialize.
-  inline {1} Dkc.Dkc.encrypt.
-  inline {1} AdvGarble.Adv(ADV).garble_queries.
-  inline {1} AdvGarble.Adv(ADV).garble_answer.
-  inline {1} AdvGarble.Adv(ADV).query1.
-  inline {1} AdvGarble.Adv(ADV).query2.
-  inline {1} AdvGarble.Adv(ADV)._query1.
-  inline {1} AdvGarble.Adv(ADV)._query2.
-  inline {1} AdvGarble.Adv(ADV).garb.
-  inline {1} AdvGarble.Adv(ADV).garbD.
-  inline {2} Garble.PrvInd(RandGarble).garb.
-  inline {2} Garble.PrvInd(RandGarble).get_challenge.
-  inline {2} RandGarble.gen.
+  inline {1} GameAda(DKC.Dkc, ADV).A.work.
+  inline {1} AdvAda(ADV, DKC.Dkc).work.
+  inline {1} AdvAda(ADV, DKC.Dkc).garble.
+  inline {1} DKC.Dkc.preInit.
+  inline {1} DKC.Dkc.get_challenge.
+  inline {1} DKC.Dkc.initialize.
+  inline {1} DKC.Dkc.encrypt.
+  inline {1} AdvAda(ADV, DKC.Dkc).query.
+  inline {1} AdvAda(ADV, DKC.Dkc).garb.
+  inline {1} AdvAda(ADV, DKC.Dkc).garbD.
+  inline {2} Garble.PrvInd(RandGarble2).garb.
+  inline {2} Garble.PrvInd(RandGarble2).get_challenge.
+  inline {2} RandGarble2.gen.
 
   swap{1} 7 -6.
 
-  app 1 1 : (AdvGarble.Adv.query{1} = query{2}).
-  call ((glob ADV){1} = (glob ADV){2}) (res{1}=res{2} /\ (glob ADV){1} = (glob ADV){2}).
-    fun true;trivial.
+  app 1 1 : (AdvAda.query{1} = query{2}/\DKC.Dkc.b{1}).
+    call ((glob ADV){1} = (glob ADV){2}) (res{1}=res{2} /\ (glob ADV){1} = (glob ADV){2}).
+      fun true;trivial.
   skip;trivial.
   
   case (Garble.queryValid query{2}).
 
-  rcondt {1} 18;[admit|].
-  rcondt {1} 33.
-  intros &m;kill 26!7. kill 1!24.
-wp;skip;trivial.
-wp.
-while true (AdvGarble.Adv.n + AdvGarble.Adv.q - 1 - AdvGarble.Adv.g). intros z.
-wp.
-kill 1!4.
-skip.
-trivial.
-if.
+  (*VALID*)
+  rcondt {1} 18;[intros _;wp;rnd;wp;rnd;rnd;skip;trivial|].
   rcondt {2} 1;[intros &m;skip;trivial|].
+  wp.
+  call ((glob ADV){1} = (glob ADV){2}/\answer{1}=answer{2}) (res{1}=res{2});[fun true;trivial|].
+  wp.
+  app 26 15 : (
+    (glob ADV){1} = (glob ADV){2} /\
+    AdvAda.xx{1} = xx{2} /\
+    AdvAda.t{1} = t{2}/\
+    AdvAda.n{1} = n{2}/\
+    AdvAda.m{1} = m{2}/\
+    AdvAda.q{1} = q{2}/\
+    AdvAda.aa{1} = aa{2}/\
+    AdvAda.bb{1} = bb{2}/\
+    AdvAda.fc{1} = f{2}/\
+    (AdvAda.c{1} = DKC.Dkc.b{1}) = PrvInd.b{2}/\
+    AdvAda.xc{1} = x{2}
+  ).
+  wp.
+  app 24 13 : (
+    (glob ADV){1} = (glob ADV){2} /\
+    AdvAda.xx{1} = xx{2} /\
+    AdvAda.t{1} = t{2}/\
+    AdvAda.n{1} = n{2}/\
+    AdvAda.m{1} = m{2}/\
+    AdvAda.q{1} = q{2}/\
+    AdvAda.aa{1} = aa{2}/\
+    AdvAda.bb{1} = bb{2}/\
+    AdvAda.fc{1} = f{2}/\
+    (AdvAda.c{1} = DKC.Dkc.b{1}) = PrvInd.b{2}/\
+    AdvAda.xc{1} = x{2}
+  ).
   
+  admit.
+  while (
+    (glob ADV){1} = (glob ADV){2} /\
+    AdvAda.xx{1} = xx{2} /\
+    AdvAda.t{1} = t{2}/\
+    AdvAda.n{1} = n{2}/\
+    AdvAda.m{1} = m{2}/\
+    AdvAda.q{1} = q{2}/\
+    AdvAda.aa{1} = aa{2}/\
+    AdvAda.bb{1} = bb{2}/\
+    AdvAda.fc{1} = f{2}/\
+    AdvAda.xc{1} = x{2}/\
+    (AdvAda.c{1} = DKC.Dkc.b{1}) = PrvInd.b{2}/\
+    AdvAda.i{1} = i{2}
+  ).
+  wp.
+  app 1 1 : (
+    (glob ADV){1} = (glob ADV){2} /\
+    AdvAda.xx{1} = xx{2} /\
+    AdvAda.t{1} = t{2}/\
+    AdvAda.n{1} = n{2}/\
+    AdvAda.m{1} = m{2}/\
+    AdvAda.q{1} = q{2}/\
+    AdvAda.aa{1} = aa{2}/\
+    AdvAda.bb{1} = bb{2}/\
+    AdvAda.fc{1} = f{2}/\
+    AdvAda.xc{1} = x{2}/\
+    (AdvAda.c{1} = DKC.Dkc.b{1}) = PrvInd.b{2}/\
+    AdvAda.i{1} = i{2}
+  );(if;[progress|wp;rnd;skip;progress|skip;progress]).
+  wp;skip;progress.
+  
+  app 2 0 : (
+    (glob ADV){1} = (glob ADV){2} /\
+    AdvAda.xx{1} = xx{2} /\
+    AdvAda.t{1} = t{2}/\
+    AdvAda.n{1} = n{2}/\
+    AdvAda.m{1} = m{2}/\
+    AdvAda.q{1} = q{2}/\
+    AdvAda.aa{1} = aa{2}/\
+    AdvAda.bb{1} = bb{2}/\
+    AdvAda.fc{1} = f{2}/\
+    AdvAda.xc{1} = x{2}/\
+    let (g, e, d) = garble xx{2} f{2} in getG g = AdvAda.pp{1}/\
+    (AdvAda.c{1} = DKC.Dkc.b{1}) = PrvInd.b{2}).
+    admit. (*While one sided*)
+  skip.
+  delta garble.
+  progress. trivial.
+
+  (*INVALID*)
+  rcondf {1} 18;[intros _;wp;rnd;wp;rnd;rnd;skip;trivial|].
+  rcondf {1} 26. admit.
+  rcondf {2} 1;[intros &m;skip;trivial|].
+  wp.
+  rnd.
+  kill{1} 1!25.
+  skip;trivial.
+    admit.
 save.
