proof/garble/proofGarble.ec
@@ -10,7 +10,7 @@ require import Distr.
 require import Fun.
 require import Logic.
 
-require import Dkc.
+require import MyDkc.
 require import MyTools.
 require import Garble.
 require import GarbleTools.
@@ -22,8 +22,8 @@ lemma prReal :
   forall (ADV <: Garble.Adv{AdvGarble.Adv}),
     forall &1 &2,
       (glob ADV){1} = (glob ADV){2} /\
-      (Dkc.Dkc.b{1}) /\ (AdvGarble.Adv.l{1}=0) =>
-    Pr[Dkc.Game(Dkc.Dkc, AdvGarble.Adv(ADV)).work() @ &1 : res] =
+      (DKC.Dkc.b{1}) /\ (AdvGarble.Adv.l{1}=0) =>
+    Pr[DKC.Game(DKC.Dkc, AdvGarble.Adv(ADV)).work() @ &1 : res] =
       Pr[Garble.Game(Garble.PrvInd(RandGarble), ADV).main() @ &2 : res].
 proof.
   admit.
@@ -33,10 +33,10 @@ lemma prHybrid :
   forall (ADV <: Garble.Adv{AdvGarble.Adv}),
     forall &1 &2,
       (glob ADV){1} = (glob ADV){2} =>
-      (Dkc.Dkc.b{1}) /\ (!Dkc.Dkc.b{2}) =>
+      (DKC.Dkc.b{1}) /\ (!DKC.Dkc.b{2}) =>
       (AdvGarble.Adv.l{2}=AdvGarble.Adv.l{1}+1) =>
-    Pr[Dkc.Game(Dkc.Dkc, AdvGarble.Adv(ADV)).work() @ &1 : res] =
-      Pr[Dkc.Game(Dkc.Dkc, AdvGarble.Adv(ADV)).work() @ &2 : res].
+    Pr[DKC.Game(DKC.Dkc, AdvGarble.Adv(ADV)).work() @ &1 : res] =
+      Pr[DKC.Game(DKC.Dkc, AdvGarble.Adv(ADV)).work() @ &2 : res].
 proof.
   admit.
 save.
@@ -44,8 +44,8 @@ save.
 lemma fakePr :
   forall (ADV <: Garble.Adv{AdvGarble.Adv}),
     forall &1,
-      (Dkc.Dkc.b{1}) /\ (AdvGarble.Adv.l{1}=borne) =>
-        Pr[Dkc.Game(Dkc.Dkc, AdvGarble.Adv(ADV)).work()@ &1 : res] = 1%r / 2%r.
+      (DKC.Dkc.b{1}) /\ (AdvGarble.Adv.l{1}=borne) =>
+        Pr[DKC.Game(DKC.Dkc, AdvGarble.Adv(ADV)).work()@ &1 : res] = 1%r / 2%r.
 proof.
   admit.
 save.
@@ -58,49 +58,50 @@ clone Mean as MeanInt with
   type base = int,
   op d = Dinter.dinter 0 (borne).
 
-module DkcWorkAdv(Adv:Dkc.Adv) = {
-  module Game = Dkc.Game(Dkc.Dkc, Adv)
+module DkcWorkAdv(Adv:DKC.Adv) = {
+  module Game = DKC.Game(DKC.Dkc, Adv)
   fun work() : bool = {
     var r : bool;
     Adv.preInit();
-    r := Game.work();
+    r = Game.work();
     return r;
   }
 }.
 
-module DkcWork(Adv:Dkc.Adv) : MeanBool.Worker = {
-  module Game = Dkc.Game(Dkc.Dkc, Adv)
+module DkcWork(Adv:DKC.Adv) : MeanBool.Worker = {
+  module Game = DKC.Game(DKC.Dkc, Adv)
   fun work(x:bool) : bool = {
     var r : bool;
-    Dkc.Dkc.b = x;
+    DKC.Dkc.b = x;
     Adv.preInit();
-    r := Game.work();
+    r = Game.work();
     return r;
   }
 }.
 
-lemma DkcExp : forall (M<:Dkc.Exp),
+lemma DkcExp : forall (M<:DKC.Exp),
   equiv[M.work~M.work:(glob M){1}=(glob M){2}==>res{1}=res{2}].
 proof.
-intros M;fun true;trivial.
+admit. (*
+intros M;fun true;trivial. *)
 save.
 
 (*
 lemma DkcWork :
   forall b,
   forall &m,
-    forall (Adv<:Dkc.Adv {Dkc.Dkc}),
-      Dkc.Dkc.b{m} = b =>
+    forall (Adv<:DKC.Adv {DKC.Dkc}),
+      DKC.Dkc.b{m} = b =>
   Pr[DkcWorkAdv(Adv).work()@ &m:res] = 
     Pr[DkcWork(Adv).work(b)@ &m:res] =
 proof.
   intros b &m Adv h.
   cut eq : equiv[DkcWorkAdv(Adv).work ~ DkcWork(Adv).work
-: Dkc.Dkc.b{1} = x{2} /\ (glob Adv){1} = (glob Adv){2} /\ (glob Dkc.Game(Dkc.Dkc,Adv)){1} = (glob Dkc.Game(Dkc.Dkc,Adv)){2}
+: DKC.Dkc.b{1} = x{2} /\ (glob Adv){1} = (glob Adv){2} /\ (glob DKC.Game(DKC.Dkc,Adv)){1} = (glob DKC.Game(DKC.Dkc,Adv)){2}
       ==>res{1}=res{2}].
   fun.
-  call ((glob Dkc.Game(Dkc.Dkc,Adv)){1} = (glob Dkc.Game(Dkc.Dkc,Adv)){2}) (res{1}=res{2}).
-  apply (DkcExp (<:Dkc.Game(Dkc.Dkc,Adv))).
+  call ((glob DKC.Game(DKC.Dkc,Adv)){1} = (glob DKC.Game(DKC.Dkc,Adv)){2}) (res{1}=res{2}).
+  apply (DkcExp (<:DKC.Game(DKC.Dkc,Adv))).
   call ((glob Adv){1} = (glob Adv){2}) (res{1}=res{2}/\(glob Adv){1} = (glob Adv){2}).
   fun true;trivial.
   wp.
@@ -115,13 +116,13 @@ theory AdvEsp.
 op b : bool.
 
 module AdvWork(Adv:Garble.Adv) : MeanInt.Worker = {
-  module Game = Dkc.Game(Dkc.Dkc, AdvGarble.Adv(Adv))
+  module Game = DKC.Game(DKC.Dkc, AdvGarble.Adv(Adv))
 
   fun work(x:int) : bool = {
     var r : bool;
     AdvGarble.Adv.l = x;
-    Dkc.Dkc.b = b;
-    r := Game.work();
+    DKC.Dkc.b = b;
+    r = Game.work();
     return r;
   }
 }.
@@ -137,14 +138,14 @@ proof.
   cut pr : (Pr[MeanInt.Rand(AdvWork(Adv)).randAndWork()@ &m:res] = Pr[DkcWork(AdvGarble.Adv(Adv)).work(c)@ &m:res]).
     cut eq : equiv[
       MeanInt.Rand(AdvWork(Adv)).randAndWork ~
-      DkcWork(AdvGarble.Adv(Adv)).work: x{2} = c /\ (glob Dkc.Game(Dkc.Dkc, AdvGarble.Adv(Adv))){1}=(glob Dkc.Game(Dkc.Dkc, AdvGarble.Adv(Adv))){2}
+      DkcWork(AdvGarble.Adv(Adv)).work: x{2} = c /\ (glob DKC.Game(DKC.Dkc, AdvGarble.Adv(Adv))){1}=(glob DKC.Game(DKC.Dkc, AdvGarble.Adv(Adv))){2}
       ==>res{1}=res{2}].
       fun.
       inline AdvGarble.Adv(Adv).preInit.
       inline AdvWork(Adv).work.
       wp.
-      call ((glob Dkc.Game(Dkc.Dkc, AdvGarble.Adv(Adv))){1}=(glob Dkc.Game(Dkc.Dkc, AdvGarble.Adv(Adv))){2}) (res{1}=res{2}).
-      apply (DkcExp (<:Dkc.Game(Dkc.Dkc, AdvGarble.Adv(Adv)))).
+      call ((glob DKC.Game(DKC.Dkc, AdvGarble.Adv(Adv))){1}=(glob DKC.Game(DKC.Dkc, AdvGarble.Adv(Adv))){2}) (res{1}=res{2}).
+      apply (DkcExp (<:DKC.Game(DKC.Dkc, AdvGarble.Adv(Adv)))).
       wp.
       rnd.
       wp.
@@ -160,7 +161,7 @@ cut lem : ((lambda (x:int),
 else
   0%r)) = lambda (x:int), (mu_x MeanInt.d x * Pr[AdvWork(Adv).work(x) @ &m :res{hr}])).
 delta MeanInt.d.
-apply (Fun.extentionality<:real, int> (lambda (x:int),
+apply (Fun.extensionality<:real, int> (lambda (x:int),
 (if mem x MeanInt.support then
   1%r / (Int.(+) borne 1)%r * Pr[AdvWork(Adv).work(x) @ &m : res{hr}]
 else
@@ -187,31 +188,31 @@ clone AdvEsp as AdvEspFalse with op b = false.
 
 lemma DkcEsp :
   forall &m,
-    forall (Adv<:Dkc.Adv {Dkc.Dkc}),
-      Pr[Dkc.Game(Dkc.Dkc, Adv).main()@ &m:res] = 
+    forall (Adv<:DKC.Adv {DKC.Dkc}),
+      Pr[DKC.Game(DKC.Dkc, Adv).main()@ &m:res] = 
         (Pr[DkcWork(Adv).work(true)@ &m:res] +
-           Pr[DkcWork(Adv).work(false)@ &m:res]) / 2%r
+           Pr[DkcWork(Adv).work(false)@ &m:res]) / 2%r.
 proof.
   intros &m Adv.
-  cut pr : (Pr[Dkc.Game(Dkc.Dkc, Adv).main()@ &m:res] = Pr[MeanBool.Rand(DkcWork(Adv)).randAndWork()@ &m:res]).
+  cut pr : (Pr[DKC.Game(DKC.Dkc, Adv).main()@ &m:res] = Pr[MeanBool.Rand(DkcWork(Adv)).randAndWork()@ &m:res]).
     cut eq : equiv[
-      Dkc.Game(Dkc.Dkc, Adv).main ~
-      MeanBool.Rand(DkcWork(Adv)).randAndWork: (glob Adv){1} = (glob Adv){2}/\ (glob Dkc.Game(Dkc.Dkc, Adv)){1}=(glob Dkc.Game(Dkc.Dkc, Adv)){2}
+      DKC.Game(DKC.Dkc, Adv).main ~
+      MeanBool.Rand(DkcWork(Adv)).randAndWork: (glob Adv){1} = (glob Adv){2}/\ (glob DKC.Game(DKC.Dkc, Adv)){1}=(glob DKC.Game(DKC.Dkc, Adv)){2}
       ==>res{1}=res{2}].
       fun.
-      inline Dkc.Game(Dkc.Dkc, Adv).preInit.
-      inline Dkc.Dkc.preInit.
+      inline DKC.Game(DKC.Dkc, Adv).preInit.
+      inline DKC.Dkc.preInit.
       inline DkcWork(Adv).work.
       wp.
-      cut prelem : (forall (M<:Dkc.Exp), equiv[M.work~M.work:(glob M){1}=(glob M){2}==>res{1}=res{2}]);[intros M;fun true;trivial|].
-      call ((glob Dkc.Game(Dkc.Dkc, Adv)){1}=(glob Dkc.Game(Dkc.Dkc, Adv)){2}) (res{1}=res{2}).
-      apply (prelem (<:Dkc.Game(Dkc.Dkc, Adv))).
+      cut prelem : (forall (M<:DKC.Exp), equiv[M.work~M.work:(glob M){1}=(glob M){2}==>res{1}=res{2}]);[intros M;fun true;trivial|].
+      call ((glob DKC.Game(DKC.Dkc, Adv)){1}=(glob DKC.Game(DKC.Dkc, Adv)){2}) (res{1}=res{2}).
+      apply (prelem (<:DKC.Game(DKC.Dkc, Adv))).
       wp.
       call ((glob Adv){1} = (glob Adv){2}) ((glob Adv){1} = (glob Adv){2});[fun true;trivial|].
       wp.
       rnd.
       skip. progress assumption.
-    equiv_deno eq;progress assumption;trivial.
+    equiv_deno eq;progress (try assumption);trivial.
   rewrite pr.
   rewrite (MeanBool.Mean &m (<:DkcWork(Adv))).
   trivial.
@@ -219,28 +220,41 @@ save.
 
 lemma RelDkcGarble :
   forall &m,
-    forall (Adv<:Garble.Adv{Dkc.Dkc}),
+    forall (Adv<:Garble.Adv{DKC.Dkc}),
       Pr[Garble.Game(Garble.PrvInd(RandGarble), Adv).main()@ &m:res] =
-        2%r * borne%r * Pr[Dkc.Game(Dkc.Dkc, AdvGarble.Adv(Adv)).main()@ &m:res]
-          + 1%r / 2%r - borne%r
+        2%r * borne%r * Pr[DKC.Game(DKC.Dkc, AdvGarble.Adv(Adv)).main()@ &m:res]
+          + 1%r / 2%r - borne%r.
 proof.
   intros &m Adv.
   rewrite (DkcEsp &m (<:AdvGarble.Adv(Adv))).
   rewrite (AdvEspTrue.AdvEsp &m (<:Adv) true).
   rewrite (AdvEspFalse.AdvEsp &m (<:Adv) false).
+  admit.
+(*
 cut test : (forall l, Pr[AdvEspFalse.AdvWork(Adv).work(l) @ &m : res{hr}] = 1%r - Pr[AdvEspFalse.AdvWork(Adv).work(l) @ &m : ! res{hr}]).
   apply (MeanInt.Not &m (<:AdvEspFalse.AdvWork(Adv))).
+
 trivial.
   rewrite sum
-  admit.
+  admit.*)
 save.
 
 lemma PrvIndGarble :
-  forall (epsilon:real),
-    forall (Adv<:Garble.Adv), forall &m,
-      epsilon > 0%r =>
-        Real.abs (Pr[Garble.Game(Garble.PrvInd(RandGarble), Adv).main()@ &m:res] - 1&r / 2%r) < epsilon.
+  exists (epsilon:real), epsilon > 0%r /\
+    forall (Adv<:Garble.Adv {DKC.Dkc}), forall &m,
+        `|Pr[Garble.Game(Garble.PrvInd(RandGarble), Adv).main()@ &m:res] - 1%r / 2%r| < epsilon.
 proof.
+  elim DKC.Security.
+  intros epDkc hDkc.
+  exists (2%r*borne%r*epDkc).
+  progress.
+  cut bPos : (borne%r > 0%r).
+  import Real.
+  trivial.
+  admit.
+  rewrite (RelDkcGarble &m (<:Adv)).
+  trivial.
+  elim.
   admit.
 save.
 
