proof/garble/myDkc.ec
@@ -1,0 +1,8 @@
+require Dkc.
+require import Int.
+
+op myK : int.
+
+axiom mykVal : myK > 1.
+
+clone Dkc.DKC as DKC with op k = myK.
