proof/myRand.ec
@@ -1,0 +1,16 @@
+require import Bool.
+require import Bitstring.
+require import Pair.
+require import Distr.
+require import Int.
+
+theory Dbitstringlast.
+  op dbitstringlast : int -> bool -> bitstring distr.
+(*
+  op _internal = Dprod.dprod (Dbitstring.dbitstring (k-1)) (Dunit.dunit v).
+*)
+
+  axiom mu_weight : forall (k:int) v, k > 1 =>
+     mu_weight (dbitstringlast k v) = 1%r.
+    
+end Dbitstringlast.
