proof/myset.ec
@@ -1,0 +1,29 @@
+require import Set.
+require import Real.
+require import Distr.
+
+op fold_right : ('a -> 'b -> 'b) -> 'b -> 'a set -> 'b.
+axiom fold_nil: forall (e:'b) (f:'a -> 'b -> 'b),
+  fold_right f e Set.empty = e.
+axiom fold_cons: forall (e:'b) (f:'a -> 'b -> 'b) xs,
+  let x = Set.pick xs in
+  fold_right f e xs = f x (fold_right f e (Set.rm x xs)).
+axiom fold_cons2: forall (e:'b) (f:'a -> 'b -> 'b) xs x,
+  fold_right f e (add x xs) = f x (fold_right f e xs).
+
+op sum(f:'a -> real, s:'a set) : real =
+  fold_right (lambda (x:'a, sum:real), sum + f x) (0%r) s.
+
+lemma sum_in :
+  forall (f:'a -> real) (s:'a set),
+  sum f s = sum (lambda x, if mem x s then f x else 0%r) s.
+proof.
+admit.
+save.
+
+lemma sum_add :
+  forall (f:'a -> real) (g:'a -> real) (s:'a set),
+  (sum f s) + (sum g s) = sum (lambda x, f x + g x) s.
+proof.
+admit.
+save.
